\documentclass{article}

\usepackage{amsmath}

\begin{document}

Leakage term
	\begin{equation}
		-k_L s_L B_E \frac{1 - \frac{C}{C_{La}}}{C + s_L}
	\end{equation}
	\\
	\\
	\begin{equation}
		\frac{dC}{dt} =  sr_{C} -  k_C \frac{C}{C+k_M} \frac{[MMP]}{[MMP] +s_{C}}
	\end{equation}

	\begin{equation}
		\frac{d[MMP]}{dt} =  \alpha_{MMP} M_I \frac{F_\alpha}{F_\alpha + s_{MMP}} - \mu_{MMP}[MMP] + sr_{MMP}
	\end{equation}
	\\
	\\
	\begin{equation}
		\frac{dC}{dt} = 0 \implies k_C  = sr_{C} \frac{C + k_M}{C} \frac{[MMP] +s_{C}}{[MMP]}
	\end{equation}

\end{document}